Concurrent allocation - example 3 - roadmap adequacy

theories/examples/concurrent_alloc.v
@@ -270,5 +270,476 @@ Section concurrent_alloc.
     cbn.
     by wp_pure ; wp_end.
   Qed.
-
 End concurrent_alloc.
+
+
+
+Section adequacy.
+
+Instance DisjointList_list_Addr : DisjointList (list Addr).
+Proof. exact (@disjoint_list_default _ _ app []). Defined.
+
+Class memory_layout `{MachineParameters} := {
+  (* Code of f *)
+  f_region_start : Addr;
+  f_start : Addr;
+  f_end : Addr;
+  f_size: (f_start + (length (check_alloc_instrs' 0 1)) = Some f_end)%a;
+  f_region_start_offset: (f_region_start + 1)%a = Some f_start;
+
+  (* adversary code *)
+  adv_region_start : Addr;
+  adv_start : Addr;
+  adv_end : Addr;
+  adv_instrs : list Word;
+  adv_size : (adv_start + (length adv_instrs) = Some adv_end)%a ;
+  adv_region_start_offset: (adv_region_start + 1)%a = Some adv_start;
+
+  (* malloc routine *)
+  l_malloc_start : Addr;
+  l_malloc_memptr : Addr;
+  l_malloc_mem_start : Addr;
+  l_malloc_end : Addr;
+
+  l_malloc_code_size :
+    (l_malloc_start + length malloc_subroutine_instrs)%a
+    = Some l_malloc_memptr;
+
+  l_malloc_memptr_size :
+    (l_malloc_memptr + 1)%a = Some l_malloc_mem_start;
+
+  l_malloc_mem_size :
+    (l_malloc_mem_start <= l_malloc_end)%a;
+
+  (* fail routine *)
+  l_assert_start : Addr;
+  l_assert_cap : Addr;
+  l_assert_flag : Addr;
+  l_assert_end : Addr;
+
+  l_assert_code_size :
+    (l_assert_start + length assert_subroutine_instrs)%a = Some l_assert_cap;
+  l_assert_cap_size :
+    (l_assert_cap + 1)%a = Some l_assert_flag;
+  l_assert_flag_size :
+    (l_assert_flag + 1)%a = Some l_assert_end;
+
+  (* link table *)
+  link_table_start : Addr;
+  link_table_end : Addr;
+
+  link_table_size :
+    (link_table_start + 2)%a = Some link_table_end;
+
+  (* adversary link table *)
+  adv_link_table_start : Addr;
+  adv_link_table_end : Addr;
+  adv_link_table_size :
+    (adv_link_table_start + 1)%a = Some adv_link_table_end;
+
+  (* disjointness of all the regions above *)
+  regions_disjoint :
+    ## [
+        finz.seq_between adv_region_start adv_end;
+        finz.seq_between f_region_start f_end;
+        finz.seq_between link_table_start link_table_end;
+        finz.seq_between adv_link_table_start adv_link_table_end;
+        finz.seq_between l_assert_start l_assert_end;
+        finz.seq_between l_malloc_mem_start l_malloc_end;
+        [l_malloc_memptr];
+        finz.seq_between l_malloc_start l_malloc_memptr
+       ]
+}.
+
+
+Definition alloc_prog `{memory_layout} : prog :=
+  {| prog_start := f_start ;
+     prog_end := f_end ;
+     prog_instrs := (check_alloc_instrs' 0 1) ;
+     prog_size := f_size |}.
+
+Definition adv_prog `{memory_layout} : prog :=
+  {| prog_start := adv_start ;
+     prog_end := adv_end ;
+     prog_instrs := adv_instrs ;
+     prog_size := adv_size |}.
+
+
+Program Definition layout `{memory_layout} : ocpl_library :=
+  {| (* malloc library *)
+     malloc_start := l_malloc_start;
+     malloc_memptr := l_malloc_memptr;
+     malloc_mem_start := l_malloc_mem_start;
+     malloc_end := l_malloc_end;
+
+     malloc_code_size := l_malloc_code_size;
+
+     malloc_memptr_size := l_malloc_memptr_size;
+
+     malloc_mem_size := l_malloc_mem_size;
+
+     (* assertion fail library *)
+     assert_start := l_assert_start;
+     assert_cap := l_assert_cap;
+     assert_flag := l_assert_flag;
+     assert_end := l_assert_end;
+
+     assert_code_size := l_assert_code_size;
+     assert_cap_size := l_assert_cap_size;
+     assert_flag_size := l_assert_flag_size;
+
+     (* disjointness of the two libraries *)
+     libs_disjoint := _
+  |}.
+Next Obligation.
+  intros.
+  pose proof (regions_disjoint) as Hdisjoint.
+  rewrite !disjoint_list_cons in Hdisjoint |- *. intros (?&?&?&?&?&?&?&?&?).
+  set_solver.
+Qed.
+Definition OCPLLibrary `{memory_layout} := library layout.
+
+
+Program Definition alloc_table `{memory_layout} : @tbl_priv alloc_prog OCPLLibrary :=
+  {| prog_lower_bound := f_region_start ;
+     tbl_start := link_table_start ;
+     tbl_end := link_table_end ;
+     tbl_size := link_table_size ;
+     tbl_prog_link := f_region_start_offset ;
+     tbl_disj := _
+  |}.
+Next Obligation.
+  intros. simpl.
+  pose proof (regions_disjoint) as Hdisjoint.
+  rewrite !disjoint_list_cons in Hdisjoint |- *. intros (?&?&?&?&?&?&?&?&?).
+  disjoint_map_to_list. set_solver.
+Qed.
+
+Program Definition adv_table `{memory_layout} : @tbl_pub adv_prog OCPLLibrary :=
+  {| prog_lower_bound := adv_region_start ;
+     tbl_start := adv_link_table_start ;
+     tbl_end := adv_link_table_end ;
+     tbl_size := adv_link_table_size ;
+     tbl_prog_link := adv_region_start_offset ;
+     tbl_disj := _
+  |}.
+Next Obligation.
+  intros. simpl.
+  pose proof (regions_disjoint) as Hdisjoint.
+  rewrite !disjoint_list_cons in Hdisjoint |- *. intros (?&?&?&?&?&?&?&?&?).
+  disjoint_map_to_list. set_solver.
+Qed.
+
+Context {Σ:gFunctors} {memg:memG Σ} {regg:regG Σ}
+  `{static_spinlock.lockG Σ, MP: MachineParameters}.
+
+Definition assertInv (layout : ocpl_library) :=
+  assert_inv (assert_start layout) (assert_flag layout) (assert_end layout).
+Definition mallocInv (layout : ocpl_library) γ :=
+  malloc_inv (malloc_start layout) (malloc_end layout) γ.
+
+Context {mem_layout:memory_layout}.
+Lemma alloc_correct (i : CoreN) γ:
+  Forall (λ w, is_cap w = false) adv_instrs →
+  (∀ (rmap : (gmap (CoreN*RegName) Word)) ,
+      dom (gset (CoreN*RegName)) rmap = (all_registers_s_core i) ∖ {[ (i, PC) ]} →
+    ⊢
+     inv flagN (assert_flag layout ↦ₐ WInt 0)
+       ∗ inv mallocN (mallocInv layout γ)
+       ∗ inv assertN (assertInv layout)
+       ∗ (i, PC) ↦ᵣ WCap RWX (prog_lower_bound alloc_table) (prog_end alloc_prog) (prog_start alloc_prog)
+       ∗ ([∗ map] r↦w ∈ rmap, r ↦ᵣ w ∗ ⌜is_cap w = false⌝)
+
+       (* P program and table *)
+       ∗ (prog_lower_bound alloc_table) ↦ₐ (WCap RO (tbl_start alloc_table) (tbl_end alloc_table) (tbl_start alloc_table))
+       ∗ ([∗ map] a↦w ∈ (tbl_region alloc_table), a ↦ₐ w)
+       ∗ ([∗ map] a↦w ∈ (prog_region alloc_prog), a ↦ₐ w)
+     -∗ WP (i, Seq (Instr Executable)) {{ v, True ∨ ⌜v = (i, FailedV)⌝ }}%I).
+Proof.
+  iIntros (Hints rmap Hdom) "(#Hinv & #Hmalloc & #Hassert & HPC & Hrmap & Hlink & Htable & Hprog)".
+
+  iDestruct (big_sepM_sep with "Hrmap") as "[Hrmap #Hrmapvalid]".
+  simpl.
+
+  (* setting up read only example program *)
+  iAssert (check_alloc_instrs (finz.seq_between f_start f_end) 0 1) with "[Hprog] "as "Hprog".
+  { rewrite /check_alloc_instrs /prog_region /= /mkregion.
+    iApply big_sepM_to_big_sepL2. apply finz_seq_between_NoDup.
+    pose proof f_size as Hsize.
+    rewrite finz_seq_between_length /finz.dist. solve_addr +Hsize.
+    iFrame. }
+
+  (* cleaning up the environment tables *)
+  rewrite /tbl_region /mkregion /=.
+  pose proof link_table_size as Hsize.
+  assert (is_Some (link_table_start + 1)%a) as [link_table_mid Hmid]. solve_addr+Hsize.
+  rewrite finz_seq_between_cons;[|solve_addr +Hsize].
+  rewrite (addr_incr_eq Hmid) /= finz_seq_between_singleton /=;[|solve_addr +Hmid Hsize].
+  iDestruct (big_sepM_insert with "Htable") as "[Hlink_table_start Htable]".
+  { rewrite lookup_insert_ne ; first done. solve_addr +Hmid. }
+  iDestruct (big_sepM_insert with "Htable") as "[Hlink_table_mid _]";auto.
+
+  (* determine malloc validity *)
+  iDestruct (simple_malloc_subroutine_valid with "[$Hmalloc]") as "#Hmalloc_val" .
+  rewrite /mallocInv /assertInv.
+
+  iApply (prog_malloc_spec with
+           "[- $Hmalloc $Hassert $Hlink $Hlink_table_start $Hlink_table_mid $Hprog $HPC $Hrmap]");auto.
+  apply ExecPCPerm_RWX.
+  instantiate (1:=f_end).
+  { split;auto
+    ; pose proof (f_region_start_offset) as HH
+    ; pose proof (f_size) as HH2.
+    solve_addr+HH.
+    split; solve_addr+HH2. }
+  { apply contiguous_between_of_region_addrs;auto. pose proof (f_size) as HH. solve_addr+HH. }
+  { apply le_addr_withinBounds'. solve_addr+Hsize Hmid. }
+  { apply le_addr_withinBounds'. solve_addr+Hsize Hmid. }
+  { solve_addr. }
+Qed.
+
+
+Theorem alloc_adequacy
+    (m m': Mem) (reg reg': Reg) (es: list cap_lang.expr) (γ : gname) (i j : CoreN):
+
+
+  (* Machine with 2 cores identified by {0, 1} *)
+  machine_base.CoreNum = 2 ->
+  i = core_zero ->
+  j = (i^+1)%f ->
+
+  with_lib.is_initial_memory_with_adv alloc_prog adv_prog OCPLLibrary
+    alloc_table adv_table m →
+  with_lib.is_initial_registers alloc_prog OCPLLibrary alloc_table reg i →
+  with_lib.is_initial_registers_adv adv_prog OCPLLibrary adv_table reg j →
+  Forall (λ w, is_cap w = false) (prog_instrs adv_prog) →
+
+  rtc (@erased_step cap_lang) (init_cores, (reg, m)) (es, (reg', m')) →
+  (∀ w, m' !! l_assert_flag = Some w → w = WInt 0%Z).
+Proof.
+  intros Hn_cores Hi Hj Hmem  Hreg Hreg_adv Hadv_ints Hstep.
+  apply erased_steps_nsteps in Hstep as (n & κs & Hstep).
+
+
+    (* We apply the Iris adequacy theorem, and we unfold the definition,
+       generate the resources and unfold the definition *)
+    (* Mostly boilerplates *)
+    apply (@wp_strong_adequacy Σ cap_lang _
+             init_cores (reg,m) n κs es (reg', m')) ; last assumption.
+    intros.
+
+    iMod (gen_heap_init (m:Mem)) as (mem_heapg) "(Hmem_ctx & Hmem & _)".
+    iMod (gen_heap_init (reg:Reg)) as (reg_heapg) "(Hreg_ctx & Hreg & _)" .
+
+    iExists NotStuck.
+    iExists (fun σ κs _ => ((gen_heap_interp σ.1) ∗ (gen_heap_interp σ.2)))%I.
+    iExists (map (fun _ => (fun _ => True)%I) all_cores).
+    iExists (fun _ => True)%I. cbn.
+    iFrame.
+
+    cbn in *.
+    rewrite /with_lib.is_initial_memory_with_adv in Hmem.
+
+    (* Split the memory *)
+    iDestruct (big_sepM_subseteq with "Hmem") as "Hmem".
+    Unshelve. 3: { exact (prog_tbl_region alloc_prog alloc_table
+                            ∪ prog_tbl_region adv_prog adv_table
+                            ∪ lib_region (pub_libs OCPLLibrary ++ priv_libs OCPLLibrary)
+                     ). }
+    { destruct Hmem as (? & ? & ? & _).
+      admit. }
+    iDestruct (big_sepM_union with "Hmem") as "[Hmem_prog Hmem_lib]".
+    { cbn ; destruct Hmem as (?&?&?&?&?&?&?); eauto.
+      rewrite /lib_region /= in H3,H4,H5,H6. eauto.
+      admit.
+    }
+    iDestruct (big_sepM_union with "Hmem_prog") as "[Hmem_alloc Hmem_adv]".
+    { cbn. destruct Hmem as (?&?&?&?&?&?&?); eauto. }
+    iDestruct (big_sepM_union with "Hmem_lib") as "[Hmem_lib_malloc Hmem_lib_assert]".
+    { cbn. destruct Hmem as (?&?&?&?&?&?&?); eauto.
+      by rewrite /lib_region /= map_union_empty in H6.
+    }
+    rewrite map_union_empty.
+    cbn.
+    rewrite /malloc_library_content /=.
+    rewrite /assert_library_content /=.
+
+
+
+
+    (* Allocation of all the required invariants *)
+    (* invariant malloc *)
+    iMod (inv_alloc
+            mallocN
+            ⊤ (mallocInv layout γ)
+           with "[Hmem_lib_malloc]") as "#Hinv_malloc".
+    { iNext. rewrite /mallocInv /malloc_inv.
+      simpl.
+    iDestruct (big_sepM_union with "Hmem_lib_malloc") as "[Hmem_lib_malloc Hmalloc_mem_pool]".
+    { admit. }
+    iDestruct (big_sepM_union with "Hmem_lib_malloc") as "[Hmalloc_prog Hmalloc_cap]".
+    { admit. }
+
+    iSplitL "Hmalloc_prog".
+    { admit. }
+    (* TODO the specification of malloc_library_content needs to be updated,
+       because it doesn't involve the lock *)
+    iSplitL "Hmalloc_cap".
+    { admit. }
+    iSplitR.
+    { admit. }
+    rewrite /static_spinlock.is_lock.
+    iLeft.
+    iSplitR.
+    { admit. }
+    iSplitL.
+    { iExists _. admit. }
+    rewrite /static_spinlock.locked.
+    (* iMod (own_alloc _ _ (excl.Excl ())) as (γ) "Hld". ; first done. *)
+    admit.
+    }
+
+
+    iDestruct (big_sepM_union with "Hmem_lib_assert") as "[Hmem_assert Hmem_flag]".
+    { admit. }
+    (* invariant flag *)
+    iMod (inv_alloc
+            flagN
+            ⊤ (assert_flag layout ↦ₐ WInt 0)
+           with "[Hmem_flag]") as "#Hinv_flag".
+    { iNext.
+      rewrite /assert_flag ; simpl.
+      iDestruct ( big_sepM_insert with "Hmem_flag" ) as "[flag _]".
+      { set_solver. }
+      iFrame.
+    }
+    (* invariant assert *)
+    iMod (inv_alloc
+            assertN
+            ⊤ (assertInv layout)
+           with "[Hmem_assert]") as "#Hinv_assert".
+    { iNext.
+      rewrite /assertInv /assert_inv /=; simpl.
+      admit.
+    }
+
+    iModIntro.
+    iSplitL.
+    (** For all cores, prove that it executes completely and safely *)
+    {
+      (* Since we have a machine with 2 cores, split the list into 2 WP *)
+      unfold CoreN in i,j,Hi,Hj.
+      rewrite /init_cores /all_cores.
+      rewrite /core_zero in Hi.
+      assert (Hn_cores': (BinIntDef.Z.to_nat machine_base.CoreNum) = 2%nat) by lia.
+      rewrite Hn_cores' ; cbn.
+      assert (Hcores: i ≠ j).
+      { solve_finz. }
+      rewrite <- Hi ; rewrite <- Hj ; clear Hi Hj.
+      fold CoreN in i,j.
+
+      (* We separate the registers into two sets of registers:
+         - the registers for i
+         - the registers for j
+       *)
+      rewrite /with_lib.is_initial_registers in Hreg, Hreg_adv.
+      destruct Hreg as (Hreg1_some & Hreg1_valid).
+      destruct Hreg_adv as (Hreg2_some & Hreg2_valid).
+      set (rmap_i := @set_map _ _ _ _ _ _ _
+                       (@gset_union (CoreN * RegName) _ _)
+                       (fun r : RegName => (i,r)) all_registers_s).
+      set (rmap_j := @set_map _ _ _ _ _ _ _
+                       (@gset_union (CoreN * RegName) _ _)
+                       (fun r : RegName => (j,r)) all_registers_s).
+      set (Pi:= (fun (v : (CoreN * RegName) * Word) => (fst (fst v)) = i )).
+      set (Pj:= (fun (v : (CoreN * RegName) * Word) => (fst (fst v)) = j )).
+      set (NPi := (fun (v : (CoreN * RegName) * Word) => (fst (fst v)) ≠ i )).
+      set (NPj := (λ v : CoreN * RegName * Word, (¬ Pj v)%type)).
+
+      (* replace reg with *)
+      (*   (filter Pi reg ∪ *)
+      (*      filter NPi reg) by set_solver. *)
+      (* assert (dom _ ( filter Pi reg ) = rmap_i). *)
+      (* { set_solver. } *)
+      (* set (regs_ni := filter NPi reg). *)
+      (* replace regs_ni with *)
+      (*   (filter Pj regs_ni ∪ *)
+      (*      filter NPj regs_ni) *)
+      (* by (by rewrite map_union_filter). *)
+      (* assert (dom _ ( filter Pj regs_ni ) = rmap_j). *)
+      (* { subst rmap_j. *)
+      (*   subst regs_ni. *)
+      (*   erewrite <- dom_filter_L. *)
+      (*   reflexivity. *)
+      (*   intros. *)
+      (*   split; intros. *)
+      (*   { destruct i0. *)
+      (*     apply elem_of_map_1 in H0. *)
+      (*     destruct H0 as (? & ? & ?). inversion H0 ; subst. *)
+      (*     destruct (decide (x = PC)) as [->|Hx] ; subst. *)
+      (*     - eexists ; split. *)
+      (*       apply map_filter_lookup_Some_2. *)
+      (*       eassumption. *)
+      (*       subst NPi ; cbn ; auto. *)
+      (*       cbn ; auto. *)
+      (*     - destruct (Hreg2_valid x) as (? & ? & _); eauto. *)
+      (*       { clear -Hx. set_solver. } *)
+      (*       eexists ; split. *)
+      (*       apply map_filter_lookup_Some_2. *)
+      (*       eassumption. *)
+      (*       subst NPi ; cbn ; auto. *)
+      (*       cbn ; auto. *)
+      (*   } *)
+      (*   { destruct H0 as (w & Hfilter & core_i0). *)
+      (*     destruct i0. *)
+      (*     cbn in core_i0. subst c. *)
+      (*     apply elem_of_map_2. *)
+      (*     apply all_registers_s_correct. *)
+      (*   } *)
+      (* } *)
+
+      (* iDestruct (big_sepM_union with "Hreg") as "[Hreg_i Hreg]". *)
+      (* { *)
+      (*   cbn. *)
+
+      (*   rewrite (map_filter_commute _ _ _ _ _ _ _ _ _ _ _ _ Pj _ NPi). *)
+      (*   rewrite (map_filter_commute _ _ _ _ _ _ _ _ _ _ _ _ NPj _ NPi). *)
+
+      (*   replace ( filter NPi (filter Pj reg) ∪ filter NPi (filter NPj reg) ) *)
+      (*     with (filter NPi ((filter Pj reg) ∪ (filter NPj reg))). *)
+      (*   2: { eapply map_filter_union. *)
+      (*        apply gmap_finmap. *)
+      (*        apply map_disjoint_filter. } *)
+      (*   replace (filter Pj reg ∪ filter NPj reg) *)
+      (*     with reg by (by rewrite map_union_filter). *)
+      (*   apply map_disjoint_filter. *)
+      (* } *)
+      (* iDestruct (big_sepM_union with "Hreg") as "[Hreg_j Hreg]". *)
+      (* { apply map_disjoint_filter. } *)
+      (* iClear "Hreg". *)
+
+      (* For each core, we prove the WP, using the specification previously
+         defined *)
+      (* iSplitL "Hmem_alloc Hreg_i". *)
+
+
+
+
+      admit. }
+
+
+    (** The invariant holds on the resulting memory *)
+    iIntros (es' t2) "%Hes %Hlength_es %Hstuck [Hreg' Hmem'] Hopt _".
+
+    iInv "Hinv_flag" as ">Hflag" "_".
+    iDestruct (gen_heap_valid m' with "Hmem' Hflag") as "#%flag".
+    iApply fupd_mask_intro_discard ; [set_solver|iPureIntro].
+    intros.
+    clear - flag H0. by simplify_map_eq.
+    Unshelve.
+Admitted.
+
+
+
+
+End adequacy.
