theories/examples/template_adequacy_concurrency.v
@@ -112,3 +112,149 @@ Definition is_initial_registers_adv
   /\ (∀ (r: RegName), (i, r) ∉ ({[ (i, PC) ]} : gset (CoreN * RegName)) →
                      ∃ (w:Word), reg !! (i, r) = Some w ∧ is_cap w = false).
 End with_adv.
+
+
+Record lib_entry := MkLibEntry {
+  lib_start : Addr;
+  lib_end : Addr;
+  lib_entrypoint : Addr;
+  lib_full_content : gmap Addr Word
+}.
+
+Definition entry_points (l: list lib_entry) : list Word :=
+  (map (λ entry, WCap E (lib_start entry) (lib_end entry) (lib_entrypoint entry)) l).
+
+Record lib := MkLib {
+  pub_libs : list lib_entry;
+  priv_libs : list lib_entry
+}.
+
+Record tbl {p : prog} {l : list lib_entry} := MkTbl {
+  prog_lower_bound : Addr ;
+  tbl_start : Addr ;
+  tbl_end : Addr ;
+  tbl_size : (tbl_start + length l)%a = Some tbl_end ;
+  tbl_prog_link : (prog_lower_bound + 1)%a = Some (prog_start p) ;
+
+  tbl_disj : mkregion tbl_start tbl_end (entry_points l) ##ₘ
+             mkregion prog_lower_bound (prog_end p) ((WCap RO tbl_start tbl_end tbl_start) :: (prog_instrs p))
+}.
+
+Definition tbl_region {p l} (t : @tbl p l) : gmap Addr Word :=
+  mkregion (tbl_start t) (tbl_end t) (entry_points l).
+Definition prog_lower_bound_region {l} (p : prog) (t : @tbl p l) : gmap Addr Word :=
+  mkregion (prog_lower_bound t) (prog_end p) ((WCap RO (tbl_start t) (tbl_end t) (tbl_start t)) :: (prog_instrs p)).
+Definition prog_tbl_region {l} (p : prog) (t : @tbl p l) : gmap Addr Word :=
+  prog_lower_bound_region p t ∪ tbl_region t.
+
+Lemma prog_lower_bound_region_cons {l} (p : prog) (t : @tbl p l) :
+  prog_lower_bound_region p t = <[(prog_lower_bound t):=WCap RO (tbl_start t) (tbl_end t) (tbl_start t)]> (prog_region p)
+  ∧ (prog_region p) !! (prog_lower_bound t) = None.
+Proof.
+  rewrite /prog_lower_bound_region /mkregion.
+  pose proof (tbl_prog_link t) as Ht.
+  destruct (decide (prog_start p = prog_end p)).
+  - rewrite e in Ht. rewrite /prog_region /mkregion finz_seq_between_singleton// e finz_seq_between_empty /=.
+    split;auto. solve_addr.
+  - pose proof (prog_size p).
+    assert (prog_start p <= prog_end p)%a.
+    { solve_addr. }
+    rewrite (finz_seq_between_cons (prog_lower_bound t));[|solve_addr].
+    simpl. rewrite (addr_incr_eq Ht) /=. split;auto.
+    rewrite /prog_region /mkregion.
+    apply not_elem_of_list_to_map.
+    rewrite fst_zip. apply not_elem_of_finz_seq_between. solve_addr.
+    rewrite finz_seq_between_length /finz.dist. solve_addr.
+Qed.
+
+Fixpoint lib_region (l : list lib_entry) : gmap Addr Word :=
+  match l with
+  | [] => ∅
+  | e :: l => (lib_full_content e) ∪ (lib_region l)
+  end.
+
+Lemma lib_region_app l1 l2 :
+  lib_region (l1 ++ l2) = lib_region l1 ∪ lib_region l2.
+Proof.
+  induction l1. by rewrite app_nil_l map_empty_union.
+  by rewrite /= IHl1 map_union_assoc.
+Qed.
+
+Definition tbl_pub (p : prog) (l : lib) := @tbl p (pub_libs l).
+Definition tbl_priv (p : prog) (l : lib) := @tbl p ((pub_libs l) ++ (priv_libs l)).
+
+Module with_lib.
+
+  Definition is_initial_registers
+    (P : prog) (Lib : lib) (P_tbl : tbl_priv P Lib) (reg: gmap (CoreN * RegName) Word) (i:CoreN):=
+    reg !! (i, PC) = Some (WCap RWX (prog_lower_bound P_tbl) (prog_end P) (prog_start P))
+    /\ (∀ (r: RegName), (i, r) ∉ ({[ (i, PC) ]} : gset (CoreN * RegName)) →
+                       ∃ (w:Word), reg !! (i, r) = Some w ∧ is_cap w = false).
+  
+  Definition is_initial_registers_adv (Adv: prog) (Lib : lib)
+    (Adv_tbl : tbl_pub Adv Lib) (reg: gmap (CoreN * RegName) Word) (i:CoreN):=
+    reg !! (i, PC) = Some (WCap RWX (prog_lower_bound Adv_tbl) (prog_end Adv) (prog_start Adv))
+    /\ (∀ (r: RegName), (i, r) ∉ ({[ (i, PC) ]} : gset (CoreN * RegName)) →
+                       ∃ (w:Word), reg !! (i, r) = Some w ∧ is_cap w = false).
+
+  (* Definition is_initial_registers_adv *)
+  (*   (P : adv_prog) (Lib : lib) (P_tbl : tbl_priv P Lib) (reg: gmap (CoreN * RegName) Word) (i:CoreN):= *)
+  (*   reg !! (i, PC) = Some (WCap RWX (prog_lower_bound P_tbl) (prog_end P) (prog_start P)) *)
+  (*   /\ (∀ (r: RegName), (i, r) ∉ ({[ (i, PC) ]} : gset (CoreN * RegName)) → *)
+  (*                      ∃ (w:Word), reg !! (i, r) = Some w ∧ is_cap w = false). *)
+
+  Definition is_initial_registers_with_adv
+    (P Adv: prog) (Lib : lib) (P_tbl : tbl_priv P Lib)
+    (Adv_tbl : tbl_pub Adv Lib) (reg: gmap (CoreN*RegName) Word)
+    (r_adv: RegName) (i:CoreN) :=
+    reg !! (i, PC) = Some (WCap RWX (prog_lower_bound P_tbl) (prog_end P) (prog_start P))
+    ∧ reg !! (i, r_adv) = Some (WCap RWX (prog_lower_bound Adv_tbl) (prog_end Adv) (prog_start Adv))
+    ∧ PC ≠ r_adv
+    ∧ (∀ (r: RegName), (i,r) ∉ ({[ (i,PC) ; (i,r_adv) ]} : gset (CoreN*RegName)) →
+                       ∃ (w:Word), reg !! (i,r) = Some w ∧ is_cap w = false).
+
+  Lemma initial_registers_full_map (P : prog) (Lib : lib)
+    (P_tbl : tbl_priv P Lib) reg (i:CoreN) :
+    is_initial_registers P Lib P_tbl reg  i →
+    (∀ r, is_Some (reg !! (i,r))).
+  Proof.
+    intros (HPC & Hothers) r.
+    destruct (decide (r = PC)) as [->|]. by eauto.
+    destruct (Hothers r) as (w & ? & ?); [| eauto]. set_solver.
+  Qed.
+
+  Lemma initial_registers_adv_full_map (P : prog) (Lib : lib)
+    (P_tbl : tbl_pub P Lib) reg (i:CoreN) :
+    is_initial_registers_adv P Lib P_tbl reg  i →
+    (∀ r, is_Some (reg !! (i,r))).
+  Proof.
+    intros (HPC & Hothers) r.
+    destruct (decide (r = PC)) as [->|]. by eauto.
+    destruct (Hothers r) as (w & ? & ?); [| eauto]. set_solver.
+  Qed.
+
+  Definition is_initial_memory (P : prog) (Lib : lib) (P_tbl : tbl_priv P Lib) (m: gmap Addr Word) :=
+    prog_tbl_region P P_tbl ⊆ m
+    ∧ lib_region ((pub_libs Lib) ++ (priv_libs Lib)) ⊆ m
+    ∧ prog_tbl_region P P_tbl ##ₘlib_region ((pub_libs Lib) ++ (priv_libs Lib))
+    ∧ lib_region (pub_libs Lib) ##ₘlib_region (priv_libs Lib).
+
+  Definition is_initial_memory_with_adv (P Adv: prog) (Lib : lib) (P_tbl : tbl_priv P Lib) (Adv_tbl : tbl_pub Adv Lib) (m: gmap Addr Word) :=
+    prog_tbl_region P P_tbl ⊆ m
+    ∧ prog_tbl_region Adv Adv_tbl ⊆ m
+    ∧ lib_region ((pub_libs Lib) ++ (priv_libs Lib)) ⊆ m
+    ∧ prog_tbl_region P P_tbl ##ₘprog_tbl_region Adv Adv_tbl
+    ∧ prog_tbl_region P P_tbl ##ₘlib_region ((pub_libs Lib) ++ (priv_libs Lib))
+    ∧ prog_tbl_region Adv Adv_tbl ##ₘlib_region ((pub_libs Lib) ++ (priv_libs Lib))
+    ∧ lib_region (pub_libs Lib) ##ₘlib_region (priv_libs Lib).
+
+  Definition initial_memory_domain (P : prog) (Lib : lib) (P_tbl : tbl_priv P Lib) : gset Addr :=
+    dom (gset Addr) (prog_tbl_region P P_tbl)
+      ∪ dom (gset Addr) (lib_region ((pub_libs Lib) ++ (priv_libs Lib))).
+
+  Definition initial_memory_domain_with_adv (P Adv: prog) (Lib : lib) (P_tbl : tbl_priv P Lib) (Adv_tbl : tbl_pub Adv Lib) : gset Addr :=
+    dom (gset Addr) (prog_tbl_region P P_tbl)
+      ∪ dom (gset Addr) (prog_tbl_region Adv Adv_tbl)
+      ∪ dom (gset Addr) (lib_region ((pub_libs Lib) ++ (priv_libs Lib))).
+
+End with_lib.
