theories/examples/template_adequacy_concurrency_ocpl.v
@@ -1,0 +1,91 @@
+From iris.algebra Require Import auth agree excl gmap gset frac.
+From iris.proofmode Require Import tactics.
+From iris.base_logic Require Import invariants.
+From iris.program_logic Require Import adequacy.
+From cap_machine Require Import
+     stdpp_extra iris_extra
+     rules logrel fundamental.
+From cap_machine.examples Require Import addr_reg_sample safe_malloc assert.
+From cap_machine.examples Require Export mkregion_helpers disjoint_regions_tactics.
+From cap_machine.examples Require Import template_adequacy_concurrency.
+
+Section ocpl.
+
+Record ocpl_library `{MachineParameters} := MkOcplLibrary {
+  (* malloc library *)
+  malloc_start : Addr;
+  malloc_memptr : Addr;
+  malloc_mem_start : Addr;
+  malloc_end : Addr;
+
+  malloc_code_size :
+    (malloc_start + length malloc_subroutine_instrs)%a
+    = Some malloc_memptr;
+
+  malloc_memptr_size :
+    (malloc_memptr + 1)%a = Some malloc_mem_start;
+
+  malloc_mem_size :
+    (malloc_mem_start <= malloc_end)%a;
+
+  (* assert library *)
+  assert_start : Addr;
+  assert_cap : Addr;
+  assert_flag : Addr;
+  assert_end : Addr;
+
+  assert_code_size :
+    (assert_start + length assert_subroutine_instrs)%a = Some assert_cap;
+  assert_cap_size :
+    (assert_cap + 1)%a = Some assert_flag;
+  assert_flag_size :
+    (assert_flag + 1)%a = Some assert_end;
+
+  (* disjointness of the two libraries *)
+  libs_disjoint : ## [
+      finz.seq_between assert_start assert_end;
+      finz.seq_between malloc_mem_start malloc_end;
+      [malloc_memptr];
+      finz.seq_between malloc_start malloc_memptr
+     ]
+}.
+
+Definition malloc_library_content `{MachineParameters} (layout : ocpl_library) : gmap Addr Word :=
+  (* code for the malloc subroutine *)
+  mkregion (malloc_start layout) (malloc_memptr layout) malloc_subroutine_instrs
+  (* Capability to malloc's memory pool, used by the malloc subroutine *)
+  ∪ list_to_map [((malloc_memptr layout), WCap RWX (malloc_memptr layout) (malloc_end layout) (malloc_mem_start layout))]
+  (* Malloc's memory pool, initialized to zero *)
+  ∪ mkregion (malloc_mem_start layout) (malloc_end layout) (region_addrs_zeroes (malloc_mem_start layout) (malloc_end layout)).
+
+Definition lib_entry_malloc `{MachineParameters} (layout : ocpl_library) : lib_entry :=
+  {| lib_start := malloc_start layout;
+     lib_end := malloc_end layout;
+     lib_entrypoint := malloc_start layout;
+     lib_full_content := malloc_library_content layout|}.
+
+(* assert library entry *)
+Definition assert_library_content `{MachineParameters} (layout : ocpl_library) : gmap Addr Word :=
+  (* code for the assert subroutine, followed by a capability to the assert flag
+     and the flag itself, initialized to 0. *)
+  mkregion (assert_start layout) (assert_cap layout) assert_subroutine_instrs
+  ∪ list_to_map [(assert_cap layout, WCap RW (assert_flag layout) (assert_end layout) (assert_flag layout))]
+  ∪ list_to_map [(assert_flag layout, WInt 0)] (* assert flag *).
+
+Definition lib_entry_assert `{MachineParameters} (layout : ocpl_library) : lib_entry :=
+  {| lib_start := assert_start layout;
+     lib_end := assert_end layout;
+     lib_entrypoint := assert_start layout;
+     lib_full_content := assert_library_content layout |}.
+
+(* full library *)
+Definition library `{MachineParameters} (layout : ocpl_library) : lib :=
+  {| priv_libs := [lib_entry_assert layout] ;
+     pub_libs := [lib_entry_malloc layout] |}.
+
+Definition assertInv `{memG Σ, regG Σ, MachineParameters} (layout : ocpl_library) :=
+  assert_inv (assert_start layout) (assert_flag layout) (assert_end layout).
+Definition mallocInv `{memG Σ, regG Σ,static_spinlock.lockG Σ, MachineParameters}
+  (layout : ocpl_library) γ :=
+  malloc_inv (malloc_start layout) (malloc_end layout) γ.
+End ocpl.
